checked-sem: initial cleanup

src/Pipit.Exp.Checked.Base.fst
@@ -15,155 +15,120 @@ module CP = Pipit.Context.Properties
 
 module PM = Pipit.Prop.Metadata
 
-// Which is better: inductive relation or recursive definition?
-// noeq
-// type check (mode: check_mode) (#t: table) (#c: context t): (#a: t.ty) -> list (row c) -> exp t c a -> Type =
-//  | CkBase:
-//           #valty: t.ty ->
-//           streams: list (row c)    ->
-//           e: exp_base t c valty    ->
-//           check mode streams (XBase e)
-//  | CkApps:
-//           #valty: t.ty ->
-//           streams: list (row c)    ->
-//           e: exp_apps t c (FTVal valty)    ->
-//           check_apps mode streams e ->
-//           check mode streams (XApps e)
-//  | CkFby1: #a: t.ty                ->
-//            start: list (row c) { List.Tot.length start <= 1 }
-//                                    ->
-//            v0: t.ty_sem a          ->
-//            e: exp t c a            ->
-//            check mode start (XFby v0 e)
-//  | CkFbyS: #a: t.ty                 ->
-//            latest: row c            ->
-//            prefix: list (row c) { List.Tot.length prefix >= 1 }
-//                                     ->
-//            v0: t.ty_sem a           ->
-//            e: exp t c a             ->
-//            check mode            prefix           e ->
-//            check mode (latest :: prefix) (XFby v0 e)
+open FStar.Squash
 
-//  | CkMu: #valty: t.ty                         ->
-//          streams: list (row c)                ->
-//          e: exp t (C.close1 c valty) valty    ->
-//          check mode streams (subst1 e (XMu e))     ->
-//          check mode streams (XMu e)
-//  | CkLet:
-//           #a: t.ty -> #b: t.ty                ->
-//           streams: list (row c)               ->
-//           e1: exp t c b                       ->
-//           e2: exp t (C.close1 c b) a          ->
-//           check mode streams (subst1 e2 e1)        ->
-//           check mode streams (XLet b e1 e2)
+[@@no_auto_projectors]
+noeq
+type check (mode: PM.check_mode) (#t: table) (#c: context t): (#a: t.ty) -> list (row c) -> exp t c a -> Type =
+ | CkBase:
+          #valty: t.ty ->
+          streams: list (row c)    ->
+          e: exp_base t c valty    ->
+          check mode streams (XBase e)
+ | CkApps:
+          #valty: t.ty ->
+          streams: list (row c)    ->
+          e: exp_apps t c (FTVal valty)    ->
+          check_apps mode streams e ->
+          check mode streams (XApps e)
+ | CkFby1: #a: t.ty                ->
+           start: list (row c) { List.Tot.length start <= 1 }
+                                   ->
+           v0: t.ty_sem a          ->
+           e: exp t c a            ->
+           check mode start (XFby v0 e)
+ | CkFbyS: #a: t.ty                 ->
+           latest: row c            ->
+           prefix: list (row c) { List.Tot.length prefix >= 1 }
+                                    ->
+           v0: t.ty_sem a           ->
+           e: exp t c a             ->
+           check mode            prefix           e ->
+           check mode (latest :: prefix) (XFby v0 e)
 
-//  | CkContract:
-//           #valty: t.ty                        ->
-//           streams: list (row c)               ->
-//           status: contract_status             ->
-//           rely: exp t c            t.propty   ->
-//           guar: exp t (valty :: c) t.propty   ->
-//           impl: exp t c            valty      ->
-//           check mode streams rely                  ->
-//           check mode streams (subst1 guar impl)    ->
-//           check mode streams impl                  ->
-//           (Some status.contract_env = mode.check_contract_env ==> bigstep_always streams rely) ->
-//           (Some status.contract_impl = mode.check_contract_impl ==> bigstep_contract_valid streams rely guar impl) ->
-//           check mode streams (XContract status rely guar impl)
+ | CkMu: #valty: t.ty                         ->
+         streams: list (row c)                ->
+         e: exp t (C.close1 c valty) valty    ->
+         check mode streams (subst1 e (XMu e))     ->
+         check mode streams (XMu e)
+ | CkLet:
+          #a: t.ty -> #b: t.ty                ->
+          streams: list (row c)               ->
+          e1: exp t c b                       ->
+          e2: exp t (C.close1 c b) a          ->
+          check mode streams (subst1 e2 e1)        ->
+          check mode streams (XLet b e1 e2)
 
-//  | CkCheck:
-//           streams: list (row c)                   ->
-//           status:  prop_status                    ->
-//           eprop:   exp t c             t.propty   ->
-//           check mode streams                eprop      ->
-//           (Some status = mode.check_assert ==> bigstep_always streams eprop) ->
-//           check mode streams (XCheck status eprop)
+ | CkContract:
+          #valty: t.ty                        ->
+          streams: list (row c)               ->
+          status: PM.contract_status             ->
+          rely: exp t c            t.propty   ->
+          guar: exp t (valty :: c) t.propty   ->
+          impl: exp t c            valty      ->
+          (PM.prop_status_contains mode status -> bigstep_always streams rely) ->
+          (PM.prop_status_contains mode PM.PSValid ->
+            bigstep_always streams rely ->
+            bigstep_always streams (subst1 guar impl)) ->
+          check mode streams rely                  ->
 
-// and check_apps (mode: check_mode) (#t: table) (#c: context t): (#a: funty t.ty) -> list (row c) -> exp_apps t c a -> Type =
-//  (* Primitives `p` are looked up in the primitive table semantics *)
-//  | CkPrim:
-//           streams: list (row c) ->
-//           p: t.prim             ->
-//           check_apps mode streams (XPrim p)
+          // if rely is true, then impl & guar check ok.
+          // this is stated as a semi-classical implication because we need the
+          // checks to be strictly smaller than the resulting check.
+          // a function impliciation here (`bigstep_always -> check & check`)
+          // makes induction difficult.
+          // note that bigstep_always is decidable.
+          either (bigstep_always streams rely -> False)
+            (check mode streams impl &
+            check mode streams (subst1 guar impl)) ->
 
-//  (* Element-wise application *)
-//  | CkApp: streams: list (row c)       ->
-//           #a: t.ty -> #b: funty t.ty  ->
-//           f: exp_apps t c (FTFun a b) ->
-//           e: exp t c  a               ->
-//           check_apps mode streams f        ->
-//           check      mode streams e        ->
-//           check_apps mode streams (XApp f e)
+          check mode streams (XContract status rely guar impl)
+
+ | CkCheck:
+          streams: list (row c)                   ->
+          status:  PM.prop_status                    ->
+          eprop:   exp t c             t.propty   ->
+          check mode streams                eprop      ->
+          (PM.prop_status_contains mode status ->
+            bigstep_always streams eprop) ->
+          check mode streams (XCheck status eprop)
+
+and check_apps (mode: PM.check_mode) (#t: table) (#c: context t): (#a: funty t.ty) -> list (row c) -> exp_apps t c a -> Type =
+ (* Primitives `p` are looked up in the primitive table semantics *)
+ | CkPrim:
+          streams: list (row c) ->
+          p: t.prim             ->
+          check_apps mode streams (XPrim p)
+
+ (* Element-wise application *)
+ | CkApp: streams: list (row c)       ->
+          #a: t.ty -> #b: funty t.ty  ->
+          f: exp_apps t c (FTFun a b) ->
+          e: exp t c  a               ->
+          check_apps mode streams f        ->
+          check      mode streams e        ->
+          check_apps mode streams (XApp f e)
 
 
+let check_all (#t: table) (#c: context t) (#a: t.ty) (mode: PM.check_mode) (e: exp t c a) =
+  forall (streams: list (row c)).
+    check mode streams e
 
-let rec check (#t: table u#i u#j) (#c: context t) (#a: t.ty) (#streams: list (row c)) (#e: exp t c a) (#v: t.ty_sem a)  (mode: PM.check_mode)
-(hBS: bigstep streams e v): Tot prop (decreases hBS) =
-  match hBS with
-  | BSBase _ _ _ _ ->
-    True
-  | BSApps _ _ _ hBSA' ->
-    check_apps mode hBSA'
-  | BSFby1 _ _ _ ->
-    True
-  | BSFbyS _ _ _ _ _ hBS' ->
-    check mode hBS'
-  | BSMu _ _ _ hBS' ->
-    check mode hBS'
-  | BSLet _ _ _ _ hBS' ->
-    check mode hBS'
-  | BSContract _ status rely guar impl _ hBSi' ->
-    // TODO: change to inductive definition so we can check rely and guar, without needing them to be evaluated in bigstep.
-    // check mode hBSr' /\
-    // check mode hBSg' /\
-    check mode hBSi' /\
-    (PM.prop_status_contains mode status ==>
-      bigstep_always streams rely) /\
-    (bigstep_always streams rely ==>
-      bigstep_always streams (subst1 guar impl))
-  | BSCheck _ status eprop _ hBS' ->
-    check mode hBS' /\
-    (PM.prop_status_contains mode status ==>
-      bigstep_always streams eprop)
+let check_apps_all (#t: table) (#c: context t) (#a: funty t.ty) (mode: PM.check_mode) (e: exp_apps t c a) =
+  forall (streams: list (row c)).
+    check_apps mode streams e
 
-and check_apps (#t: table u#i u#j) (#c: context t) (#a: funty t.ty) (#streams: list (row c)) (#e: exp_apps t c a) (#v: funty_sem t.ty_sem a) (mode: PM.check_mode) (hBSA: bigstep_apps streams e v): Tot prop (decreases hBSA) =
-  match hBSA with
-  | BSPrim _ _ -> True
-  | BSApp _ _ _ _ _ hBSA' hBS' -> check_apps mode hBSA' /\ check mode hBS'
-
-let check' (#t: table u#i u#j) (#c: context t) (#a: t.ty) (mode: PM.check_mode) (e: exp t c a) =
-  forall (streams: list (row c)) (v: t.ty_sem a) (hBS: bigstep streams e v).
-    check mode hBS
-
-let check_apps' (#t: table) (#c: context t) (#a: funty t.ty) (mode: PM.check_mode) (e: exp_apps t c a) =
-  forall (streams: list (row c)) (v: funty_sem t.ty_sem a) (hBS: bigstep_apps streams e v).
-    check_apps mode hBS
-
-let check_contract_definition (#t: table) (#c: context t) (#a: t.ty)
-  (mode: PM.check_mode)
+let contract_valid (#t: table) (#c: context t) (#a: t.ty)
   (rely: exp t c t.propty) (guar: exp t (a::c) t.propty) (impl: exp t c a) =
-  forall (streams: list (row c))
-    (vr: bool)       (hBSr: bigstep streams rely vr)
-    (vg: bool)       (hBSg: bigstep streams (subst1 guar impl) vg)
-    (vi: t.ty_sem a) (hBSi: bigstep streams impl vi).
-    check mode hBSr /\
-    check mode hBSg /\
-    check mode hBSi /\
-    (bigstep_always streams rely ==>
-      bigstep_always streams (subst1 guar impl))
-
-let bigstep_equivalent (#t: table) (#c: context t) (#a: t.ty) (e e': exp t c a): prop =
-  forall (streams: list (row c)) (v: t.ty_sem a).
-    bigstep streams e v <==> bigstep streams e' v
-
-let check_equivalent (#t: table) (#c: context t) (#a: t.ty) (m m': PM.check_mode) (e e': exp t c a): prop =
-  forall (streams: list (row c)) (v: t.ty_sem a) (hBS: bigstep streams e v) (hBS': bigstep streams e' v).
-    check m hBS <==> check m' hBS'
-
-let bless_equivalent (#t: table) (#c: context t) (#a: t.ty) (e e': exp t c a): prop =
-  bigstep_equivalent e e' /\
-  check_equivalent PM.check_mode_all  PM.check_mode_valid   e e' /\
-  check_equivalent PM.check_mode_none PM.check_mode_unknown e e'
+  forall (streams: list (row c)).
+  check PM.check_mode_unknown streams rely ==>
+  check PM.check_mode_unknown streams impl ==>
+  check PM.check_mode_unknown streams (subst1 guar impl) ==>
+  bigstep_always streams rely ==>
+    (check PM.check_mode_unknown streams rely /\
+    check PM.check_mode_unknown streams impl /\
+    check PM.check_mode_unknown streams (subst1 guar impl) /\
+    bigstep_always streams (subst1 guar impl))
 
 let rec bless (#t: table) (#c: context t) (#a: t.ty) (e: exp t c a): Tot (exp t c a) (decreases e) =
   match e with
@@ -184,9 +149,154 @@ and bless_apps (#t: table) (#c: context t) (#a: funty t.ty) (e: exp_apps t c a):
   | XPrim p -> XPrim p
   | XApp f e -> XApp (bless_apps f) (bless e)
 
-let lemma_check_bless (#t: table) (#c: context t) (#a: t.ty) (e: exp t c a { check' PM.check_mode_all e }):
-  Lemma (ensures check' PM.check_mode_valid (bless e))
-    [SMTPat (check' PM.check_mode_valid (bless e))] =
-  // TODO:ADMIT lemma
+
+let rec lemma_bless_distributes_lift (#t: table) (#c: context t) (#t1: t.ty)
+  (e1: exp t c t1)
+  (ix: C.index_insert c)
+  (t2: t.ty):
+    Lemma
+      (ensures bless (lift1' e1 ix t2) == lift1' (bless e1) ix t2)
+      (decreases e1) =
+  match e1 with
+  | XBase _ -> ()
+  | XApps ea -> lemma_bless_distributes_lift_apps ea ix t2
+  | XFby v e1' -> lemma_bless_distributes_lift e1' ix t2
+  | XMu e1' ->
+    lemma_bless_distributes_lift e1' (ix + 1) t2
+  | XLet b e1' e2' ->
+    lemma_bless_distributes_lift e1'  ix      t2;
+    lemma_bless_distributes_lift e2' (ix + 1) t2
+  | XCheck s e1' ->
+    lemma_bless_distributes_lift e1' ix t2
+  | XContract s r g i ->
+    lemma_bless_distributes_lift r  ix      t2;
+    lemma_bless_distributes_lift g (ix + 1) t2;
+    lemma_bless_distributes_lift i  ix      t2
+
+and lemma_bless_distributes_lift_apps (#t: table) (#c: context t) (#t1: funty t.ty)
+  (e1: exp_apps t c t1)
+  (ix: C.index_insert c)
+  (t2: t.ty):
+    Lemma
+      (ensures bless_apps (lift1_apps' e1 ix t2) == lift1_apps' (bless_apps e1) ix t2)
+      (decreases e1) =
+  match e1 with
+  | XPrim p -> ()
+  | XApp f e ->
+    lemma_bless_distributes_lift_apps f ix t2;
+    lemma_bless_distributes_lift e ix t2
+
+
+
+
+let rec lemma_bless_distributes_subst (#t: table) (#c: context t) (#t1: t.ty)
+  (e1: exp t c t1)
+  (ix: C.index_lookup c)
+  (e2: exp t (C.drop1 c ix) (C.get_index c ix)):
+    Lemma
+      (ensures bless (subst1' e1 ix e2) == subst1' (bless e1) ix (bless e2))
+      (decreases e1) =
+  match e1 with
+  | XBase _ -> ()
+  | XApps ea -> lemma_bless_distributes_subst_apps ea ix e2
+  | XFby v e1' -> lemma_bless_distributes_subst e1' ix e2
+  | XMu e1' ->
+    lemma_bless_distributes_lift  e2 0 t1;
+    lemma_bless_distributes_subst e1' (ix + 1) (lift1 e2 t1)
+  | XLet b e1' e2' ->
+    lemma_bless_distributes_lift  e2 0 b;
+    lemma_bless_distributes_subst e1'  ix      e2;
+    lemma_bless_distributes_subst e2' (ix + 1) (lift1 e2 b)
+  | XCheck s e1' ->
+    lemma_bless_distributes_subst e1' ix e2
+  | XContract s r g i ->
+    lemma_bless_distributes_lift  e2 0 t1;
+    lemma_bless_distributes_subst r  ix      e2;
+    lemma_bless_distributes_subst g (ix + 1) (lift1 e2 t1);
+    lemma_bless_distributes_subst i  ix      e2
+
+and lemma_bless_distributes_subst_apps (#t: table) (#c: context t) (#t1: funty t.ty)
+  (e1: exp_apps t c t1)
+  (ix: C.index_lookup c)
+  (e2: exp t (C.drop1 c ix) (C.get_index c ix)):
+    Lemma
+      (ensures bless_apps (subst1_apps' e1 ix e2) == subst1_apps' (bless_apps e1) ix (bless e2))
+      (decreases e1) =
+  match e1 with
+  | XPrim p -> ()
+  | XApp f e ->
+    lemma_bless_distributes_subst_apps f ix e2;
+    lemma_bless_distributes_subst e ix e2
+
+let rec lemma_bless_of_bigstep (#t: table) (#c: context t) (#a: t.ty) (#streams: list (row c)) (#e: exp t c a) (#v: t.ty_sem a) (hBS: bigstep streams e v):
+  Tot (bigstep streams (bless e) v)
+    (decreases hBS) =
   admit ()
 
+let rec lemma_bless_of_bigstep_always (#t: table) (#c: context t) (#streams: list (row c)) (#e: exp t c t.propty) (hB: bigstep_always streams e):
+  Tot (bigstep_always streams (bless e))
+    (decreases hB) =
+  admit ()
+
+
+let rec lemma_bigstep_always_of_bless (#t: table) (#c: context t) (#streams: list (row c)) (#e: exp t c t.propty) (hB: bigstep_always streams (bless e)):
+  Tot (bigstep_always streams e)
+    (decreases hB) =
+  admit ()
+
+let rec lemma_check_bless (#t: table) (#c: context t) (#a: t.ty) (#streams: list (row c)) (#e: exp t c a) (hC: check PM.check_mode_all streams e):
+  Tot (check PM.check_mode_valid streams (bless e))
+    (decreases hC) =
+  match hC with
+  | CkBase s b -> CkBase s b
+  | CkApps s ea hCA -> CkApps s (bless_apps ea) (lemma_check_bless_apps hCA)
+  | CkFby1 s v e1 -> CkFby1 s v (bless e1)
+  | CkFbyS l p v e1 hC1 ->
+    CkFbyS l p v _ (lemma_check_bless hC1)
+  | CkMu s e1 hC1 ->
+    lemma_bless_distributes_subst e1 0 (XMu e1);
+    CkMu s (bless e1) (lemma_check_bless hC1)
+  | CkLet s e1 e2 hC1 ->
+    lemma_bless_distributes_subst e2 0 e1;
+    CkLet s (bless e1) (bless e2) (lemma_check_bless hC1)
+  | CkContract s ps r g i hR hG hCr hCig ->
+    lemma_bless_distributes_subst g 0 i;
+
+    let hCig': either (bigstep_always s (bless r) -> False) (check PM.check_mode_valid s (bless i) & check PM.check_mode_valid s (bless (subst1 g i))) =
+      match hCig with
+      | Inl hBN -> Inl (fun hB -> hBN (lemma_bigstep_always_of_bless hB))
+      | Inr (hCi, hCg) -> Inr (lemma_check_bless hCi, lemma_check_bless hCg)
+    in
+    let hR' (pm: PM.prop_status_contains PM.check_mode_valid PM.PSValid) =
+      lemma_bless_of_bigstep_always (hR pm)
+    in
+    let hG' (pm: PM.prop_status_contains PM.check_mode_valid PM.PSValid) (hB: bigstep_always s (bless r)) =
+      lemma_bless_of_bigstep_always (hG pm (lemma_bigstep_always_of_bless hB))
+    in
+    CkContract #PM.check_mode_valid s PM.PSValid (bless r) (bless g) (bless i) hR' hG' (lemma_check_bless hCr) hCig'
+
+  | CkCheck s ps e1 hC1 hB ->
+    let hB' (pm: PM.prop_status_contains PM.check_mode_valid PM.PSValid) =
+      lemma_bless_of_bigstep_always (hB pm)
+    in
+    CkCheck s PM.PSValid (bless e1) (lemma_check_bless hC1) hB'
+
+and lemma_check_bless_apps (#t: table) (#c: context t) (#a: funty t.ty) (#streams: list (row c)) (#ea: exp_apps t c a) (hC: check_apps PM.check_mode_all streams ea):
+  Tot (check_apps PM.check_mode_valid streams (bless_apps ea))
+    (decreases hC)=
+  match hC with
+  | CkPrim s p -> CkPrim s p
+  | CkApp s f e1 hCA hC1 ->
+    CkApp s (bless_apps f) (bless e1)
+      (lemma_check_bless_apps hCA)
+      (lemma_check_bless hC1)
+
+
+let lemma_check_all_bless (#t: table) (#c: context t) (#a: t.ty) (e: exp t c a { check_all PM.check_mode_all e }):
+  Lemma (ensures check_all PM.check_mode_valid (bless e))
+    [SMTPat (check_all PM.check_mode_valid (bless e))] =
+  introduce forall streams. check PM.check_mode_valid streams (bless e)
+  with (
+    eliminate forall streams. check PM.check_mode_all streams e with streams;
+    bind_squash () (fun x -> return_squash (lemma_check_bless x))
+  )
