src/Pipit.Sugar.Check.fst
@@ -16,9 +16,9 @@ module SI  = Pipit.System.Ind
 module SX  = Pipit.System.Exp
 
 type contract (t: table) (c: context t) (a: t.ty) (rely: XCC.cexp t c t.propty) (guar: XCC.cexp t (a :: c) t.propty) =
-  impl: XCC.cexp t c a { XC.check_contract_definition PM.check_mode_all rely guar impl }
+  impl: XCC.cexp t c a { XC.contract_valid rely guar impl }
 
-let contract_of_exp1 (#t: table) (#a #b: t.ty) (r: XCC.cexp t [a] t.propty) (g: XCC.cexp t [b; a] t.propty) (i: XCC.cexp t [a] b  { XC.check_contract_definition PM.check_mode_all r g i }): contract t [a] b r g = i
+let contract_of_exp1 (#t: table) (#a #b: t.ty) (r: XCC.cexp t [a] t.propty) (g: XCC.cexp t [b; a] t.propty) (i: XCC.cexp t [a] b  { XC.contract_valid r g i }): contract t [a] b r g = i
 
 let contract_system_induct_k1' (#t: table) (#c: context t) (#a: t.ty) (r: XCC.cexp t c t.propty) (g: XCC.cexp t (a :: c) t.propty) (i: XCC.cexp t c a): prop =
   // Pipit.Exp.Causality.causal r /\
@@ -32,10 +32,10 @@ let stream_of_contract1 (#t: table) (#a #b: t.ty) (#r: XCC.cexp t [a] t.propty) 
   let impl = XC.bless contr in
   let e = XContract PM.PSUnknown rely guar impl in
   // TODO:ADMIT: requires contract_check
-  assume (XC.check_contract_definition PM.check_mode_all r g contr ==> XC.check' PM.check_mode_valid e);
+  assume (XC.contract_valid r g contr ==> XC.check' PM.check_mode_valid e);
   stream_of_exp1 e
 
-// let stream_of_contract2 (#t: table) (#a #b #c: t.ty) (contr: _contract t [a; b] c { XC.check_contract_definition PM.check_mode_all contr.rely contr.guar contr.impl }): stream t a -> stream t b -> stream t c =
+// let stream_of_contract2 (#t: table) (#a #b #c: t.ty) (contr: _contract t [a; b] c { XC.contract_valid contr.rely contr.guar contr.impl }): stream t a -> stream t b -> stream t c =
 //   let rely = XC.bless contr.rely in
 //   let guar = XC.bless contr.guar in
 //   let impl = XC.bless contr.impl in
@@ -92,7 +92,7 @@ let lemma_check_system_induct_k (#t: table) (#c: context t) (#a: t.ty) (k: nat) 
 
 let lemma_check_contract_system_induct_k1' (#t: table) (#c: context t) (#a: t.ty) (r: XCC.cexp t c t.propty) (g: XCC.cexp t (a :: c) t.propty) (i: XCC.cexp t c a):
   Lemma (requires (contract_system_induct_k1' r g i))
-        (ensures  (XC.check_contract_definition PM.check_mode_all r g i))
+        (ensures  (XC.contract_valid r g i))
         [SMTPat (contract_system_induct_k1' r g i)]
         =
     // TODO:ADMIT: induction is sound
